CP in exploration

test-suite/tabareau_vec.v
@@ -1,4 +1,5 @@
 From Equations Require Import Equations DepElimDec HSets.
+Set Universe Polymorphism.
 
 Inductive ℕ (E:Set) : Set :=
 | O : ℕ E
@@ -68,7 +69,7 @@ Proof.
   reflexivity.
 Defined.
 
-Definition sigma_eq_decomp_inv {A} {B : A -> Type} {x y : sigma A B} :
+Polymorphic Definition sigma_eq_decomp_inv {A} {B : A -> Type} {x y : sigma A B} :
   x = y -> &{ e : x.1 = y.1 & @eq_rect A x.1 B x.2 y.1 e = y.2 }.
 Proof. intros ->. exists eq_refl. simpl. exact eq_refl. Defined.
 
@@ -86,20 +87,6 @@ Arguments eissect {A B}%type_scope {f%function_scope} {_} _.
 Arguments eisadj {A B}%type_scope {f%function_scope} {_} _.
 Arguments IsEquiv {A B}%type_scope f%function_scope.
 
-Axiom cheat : forall {A}, A.
-Lemma isEquiv_cong {A B : Type} (f : A -> B) :
-  IsEquiv f -> forall x y, IsEquiv (@f_equal _ _ f x y).
-Proof.
-  intros He.
-  intros x y.
-  unshelve econstructor.
-  intros H. apply (f_equal equiv_inv) in H.
-  rewrite !eissect in H. apply H.
-  red. intros. unfold eq_ind.
-  apply cheat.
-  apply cheat.
-  apply cheat.
-Defined.
 
 
 (* Polymorphic *)
@@ -201,14 +188,6 @@ Defined.
 (*   rewrite <- (sigma_eq_2 e). rewrite e'. reflexivity. *)
 (* Defined. *)
 
-Polymorphic
-Definition ind_pack_eq_inv {A : Type}
-  {B : A -> Type} (x : A) (p q : B x) (e : @eq (sigma A (fun x => B x)) &(x & p) &(x & q))
-  (e' : eq_refl = f_equal pr1 e) : p = q.
-Proof.
-  pose proof (sigma_eq_2 e). simpl in H. destruct H. destruct e'. reflexivity.
-Defined.
-
 (* Polymorphic *)
 (* Definition ind_pack_eq_inv_refl  {A : Type} *)
 (*            {B : A -> Type} {x : &{ x : A & B x}} (e' : eq_refl = sigma_eq_1 eq_refl) : *)
@@ -230,27 +209,6 @@ Defined.
 (*   unfold eq_rect. *)
 (*   revert e'. pattern (@eq_refl A x) at 2. *)
 (* Defined. *)
-
-Polymorphic
-Definition opaque_ind_pack_eq_inv {A : Type}
-{B : A -> Type} {x : A} {p q : B x} (G : p = q -> Type) (e : &(x & p) = &(x & q))
-  (ee : eq_refl = f_equal pr1 e)
-  := G (@ind_pack_eq_inv A B x p q e ee).
-Arguments opaque_ind_pack_eq_inv : simpl never.
-
-Polymorphic
-Lemma simplify_ind_pack {A : Type}
-      (B : A -> Type) (x : A) (p q : B x) (G : p = q -> Type) :
-  (forall (e : @eq (sigma A (fun x => B x)) &(x & p) &(x & q))
-          (ee : eq_refl = f_equal pr1 e),
-          opaque_ind_pack_eq_inv G e ee) ->
-  (forall e : p = q, G e).
-Proof.
-  intros H. intros e.
-  specialize (H (ind_pack_eq e)). unfold opaque_ind_pack_eq_inv in H.
-  destruct e. simpl in H. apply (H eq_refl).
-Defined.
-Arguments simplify_ind_pack : simpl never.
 
 Polymorphic
 Definition sigma_eq_2_cong  {A A'} {B : A' -> Type} {f : A -> A'} {x y : &{ x : A & B (f x) }} :
@@ -308,31 +266,623 @@ Polymorphic
   Proof. destruct eq; auto. Defined.
 
 
+Definition sigma_eq_2_f  {A A'} {B : A' -> Type} {f : A -> A'} {x y : &{ x : A & B (f x) }} : (x = y) -> (&(f x.1 & x.2) = &(f y.1 & y.2)).
+Proof.
+  destruct x, y. simpl.
+  intros H.
+  apply sigma_eq_decomp. simpl.
+  apply sigma_eq_decomp_inv in H as [H1 H2]. simpl in *.
+  exists (f_equal f H1). simpl. destruct H1. simpl in *. exact H2.
+Defined.
+
+
+Notation " 'rew' H 'in' c " := (@eq_rect _ _ _ c _ H) (at level 20).
+
+Definition J {A} {x : A} (P : forall y : A, x = y -> Type)
+           (p : P x eq_refl) (y : A) (e : x = y) : P y e.
+  destruct e. exact p.
+Defined.
+
+Require Import Utf8.
+
+Lemma J_on_refl {A} (x y : A) (e : x = y) : J (λ (y : A) _, x = y) eq_refl y e = e.
+Proof. destruct e. constructor. Defined.
+
+Definition subst {A : Type} {x : A} {P : A -> Type} {y : A} (e : x = y) (f : P x) : P y :=
+  J (fun x _ => P x) f y e.
+
+Definition subst2 {A : Type} {x : A} {P : A -> Type} (f : P x) (y : A) (e : x = y) : P y :=
+  J (fun x _ => P x) f y e.
+
+Definition cong {A B : Type} (f : A -> B) {x y : A} (e : x = y) : f x = f y :=
+  J (fun y _ => f x = f y) (@eq_refl _ (f x)) y e.
+(* aka ap *)
+
+Lemma cong_iter {A B C} (f : A -> B) (g : B -> C) (x y : A) (e : x = y) :
+  Top.cong g (Top.cong f e) = Top.cong (fun x => g (f x)) e.
+Proof. revert y e. refine (J _ _). reflexivity. Qed.
+
+Notation " 'rew' H 'in' c " := (@subst _ _ _ _ H c) (at level 20).
+
+Notation "p =_{ P ; e } q" := (subst (P:=P) e p = q) (at level 90, format "p  =_{ P ; e }  q").
+
+Definition subst_expl {A : Type} {x : A} {P : A -> Type} {y : A} (e : x = y) (f : P x) : P y :=
+  subst e f.
+Notation " 'rewP' H 'at' P 'in' c " := (@subst_expl _ _ P _ H c) (at level 20).
+
+Polymorphic Record Equiv (A B : Type) := { equiv :> A -> B ; is_equiv :> IsEquiv equiv }.
+Arguments equiv {A B} e.
+
+Polymorphic Instance Equiv_IsEquiv {A B} (e : Equiv A B) : IsEquiv (equiv e).
+Proof. apply is_equiv. Defined.
+
+Definition inv_equiv {A B} (E: Equiv A B) : B -> A :=
+  equiv_inv (IsEquiv:=is_equiv _ _ E).
+
+Polymorphic Definition equiv_inv_equiv {A B} {E: Equiv A B} (x : A) : inv_equiv _ (equiv E x) = x :=
+  eissect x.
+Definition inv_equiv_equiv {A B} {E: Equiv A B} (x : B) : equiv E (inv_equiv _ x) = x := eisretr x.
+Definition equiv_adj {A B} {E: Equiv A B} (x : A)
+  : inv_equiv_equiv (equiv E x) = cong (equiv E) (equiv_inv_equiv x)
+  := eisadj x.
+
+Notation " X <~> Y " := (Equiv X Y) (at level 90, no associativity, Y at next level).
+
+Definition equiv_id A : A <~> A.
+Proof.
+  intros.
+  refine {| equiv a := a |}.
+  unshelve refine {| equiv_inv e := e |}.
+  - red. reflexivity.
+  - red; intros. reflexivity.
+  - intros. simpl. reflexivity.
+Defined.
+
+Axiom axiom_triangle : forall {A}, A.
+
+Definition equiv_sym {A B} : A <~> B -> B <~> A.
+Proof.
+  intros.
+  refine {| equiv a := inv_equiv X a |}.
+  unshelve refine {| equiv_inv e := equiv X e |}.
+  - red; intros. apply eissect.
+  - red; intros. apply eisretr.
+  - intros x. simpl. destruct X. simpl. unfold inv_equiv. simpl.
+    apply axiom_triangle.
+Defined.
+Axiom cheat : forall {A}, A.
+Lemma isEquiv_cong {A B : Type} (f : A -> B) :
+  IsEquiv f -> forall x y, IsEquiv (@f_equal _ _ f x y).
+Proof.
+  intros He.
+  intros x y.
+  unshelve econstructor.
+  intros H. apply (f_equal equiv_inv) in H.
+  rewrite !eissect in H. apply H.
+  red. intros. unfold eq_ind. unfold equiv_inv. destruct He.
+  apply cheat.
+  apply cheat.
+  apply cheat.
+Defined.
+
+Definition sigma_eq_2_f_inv  {A A'} {B : A' -> Type} {f : A -> A'}
+           {fequiv : IsEquiv f}
+           {x y : &{ x : A & B (f x) }} : (&(f x.1 & x.2) = &(f y.1 & y.2)) -> (x = y).
+Proof.
+  intros. apply sigma_eq_decomp_inv in H.
+  apply sigma_eq_decomp. simpl in *. destruct H.
+  revert pr2.
+  pose proof (isEquiv_cong f fequiv x.1 y.1).
+  simpl in *. pose proof (eisretr (IsEquiv := X) pr1).
+  rewrite <- H.
+  exists (equiv_inv pr1). clear -pr2.
+  revert pr2.
+  generalize (equiv_inv pr1). destruct y.
+  simpl. intros <-. trivial.
+Defined.
+
+Lemma Equiv_cong {A B : Type} (e : Equiv A B) : forall x y : A, Equiv (x = y) (equiv e x = equiv e y).
+Proof.
+  unshelve econstructor. intros H.
+  apply (f_equal (equiv e) H). apply isEquiv_cong. apply e.
+Defined.
+
+Definition square {Δ : Type} {w x y z : Δ}
+           (t : w = x) (b : y = z) (l : w = y) (r : x = z) : Type :=
+  subst (P:=fun x : Δ => x = y) t l =_{fun y : Δ => x = y;b}  r.
+
+Definition flip_square {A} {w x y z} {t b l r} (s : @square A w x y z t b l r) : square l r t b.
+Proof.
+  revert x t b l r s.
+  refine (J _ _). revert z. refine (J _ _).
+  intros l r s. unfold square in s. simpl in s.
+  revert r s. refine (J _ _).
+  revert y l. refine (J _ _).
+  unfold square. unfold subst. simpl. reflexivity.
+Defined.
+
+Lemma equiv_cong_subst {A B} (P : B -> Type) (f : A -> B)
+      (s t : A) (e : s = t) (u : P (f s))
+      (v : P (f t)) : u =_{(fun x => P (f x)); e} v <~> (u =_{P; Top.cong f e} v).
+Proof.
+  unfold Top.subst.
+  destruct e. simpl. apply equiv_id.
+Defined.
+
+Polymorphic
+  Lemma f_equal_inv' {A} {B : Type} (a b : A -> B) (u v : A)
+        (r : a u = b u)
+        (s : a v = b v)
+        (e : u = v)
+        (e' : rewP s at (fun x => b u = x) in
+            (rewP r at (fun x => x = a v) in
+                (cong a e : a u = a v)) = cong b e) :
+   rewP cong a e at (fun x => x = b u) in r =_{λ y : B, a v = y;cong b e} s.
+  Proof.
+    intros.
+    unfold subst_expl in e'.
+    apply flip_square in e'. red in e'. apply e'.
+  Defined.
+
+Polymorphic
+  Lemma f_equal_inv2 {A} {B : Type} (a b : A -> B) (u v : A)
+        (r : a u = b u)
+        (s : a v = b v)
+        (e : u = v)
+        (e' : rewP cong a e at (fun x => x = b u) in r =_{λ y : B, a v = y;cong b e} s) :
+  rewP s at (fun x => b u = x) in
+      (rewP r at (fun x => x = a v) in
+          (cong a e : a u = a v)) = cong b e.
+  Proof.
+    intros.
+    unfold subst_expl in e'.
+    apply flip_square in e'. red in e'. apply e'.
+  Defined.
+
+Polymorphic
+  Lemma f_equal_inv {A} {B : Type} (a b : A -> B) (u v : A)
+        (r : a u = b u)
+        (s : a v = b v)
+        (e : u = v)
+        (e' : rewP s at (fun x => b u = x) in
+            (rewP r at (fun x => x = a v) in
+                (cong a e : a u = a v)) = cong b e) :
+  &(u & r) = &(v & s) :> &{ x : A & a x = b x }.
+  Proof.
+    intros.
+    unfold subst_expl in e'.
+    apply flip_square in e'. red in e'.
+    destruct e. simpl in *. destruct e'. reflexivity.
+  Defined.
+
+  Lemma f_equal_inv_pack {A} {B : Type} (a b : A -> B)
+        (x y : &{ x : A & a x = b x })
+        (e : x.1 = y.1)
+        (e' : rewP y.2 at (fun z : B => b x.1 = z) in
+            (rewP x.2 at (fun z : B => z = a y.1) in
+                ((cong a e) : a x.1 = a y.1)) = cong b e) :
+    x = y.
+  Proof.
+    intros.
+    apply (f_equal_inv a b x.1 y.1) in e'. destruct x, y; auto.
+  Defined.
+
+  Lemma pack_f_equal {A} {B : A -> Type} (x : A) (p q : B x) (f : A -> A)
+        (G : forall (e : &(x & p) = &(x & q)) (e' : eq_refl = f_equal (fun x => f x.1) e), Type) :
+    (forall (e : &(x & p) = &(x & q))
+            (e' : f_equal (fun x => f x.1) eq_refl = f_equal (fun x => f x.1) e), G e e') ->
+    (forall (e : &(x & p) = &(x & q)) (e' : eq_refl = f_equal (fun x => f x.1) e), G e e').
+  Proof. intros. simpl in *. apply X. Defined.
+
+  Polymorphic Definition sigma_eq_2' {A} {B : A -> Type} {x y : &{ x : A & B x }} :
+  forall e : x = y, (@eq_rect A x.1 B x.2 y.1 (cong pr1 e)) = y.2.
+ Proof.
+  destruct e. reflexivity.
+Defined.
+
+Polymorphic
+Definition ind_pack_eq_inv {A : Type}
+  {B : A -> Type} (x y : A) (p : B x) (q : B y)
+  (e : @eq (sigma A (fun x => B x)) &(x & p) &(y & q))
+  (i : @eq A x y)
+  (e' : cong pr1 e = i) : rew i in p = q.
+Proof.
+  pose proof (sigma_eq_2' e). simpl in H. destruct e'. apply H.
+Defined.
+
+Polymorphic
+Definition opaque_ind_pack_eq_inv {A : Type} {B : A -> Type} {x y : A}
+  (i : @eq A x y) {p : B x} {q : B y} (G : p =_{B;i} q -> Type) (e : &(x & p) = &(y & q))
+  (ee : cong pr1 e = i)
+  := G (@ind_pack_eq_inv A B x y p q e i ee).
+
+Polymorphic
+Lemma simplify_ind_pack {A : Type}
+  (B : A -> Type) (x y : A) (p : B x) (q : B y) (i : x = y)
+  (G : p =_{B;i} q -> Type) :
+  (forall (exp : @eq (sigma A (fun x => B x)) &(x & p) &(y & q))
+          (ee : cong pr1 exp = i),
+          opaque_ind_pack_eq_inv i G exp ee) ->
+  (forall e : p =_{B;i} q, G e).
+Proof.
+  intros H. intros e.
+  specialize (H (make_sigma_eq i e)). unfold opaque_ind_pack_eq_inv in H.
+  destruct i, e. simpl in H. specialize (H eq_refl). simpl in G. apply H.
+Defined.
+Arguments simplify_ind_pack : simpl never.
+
+Lemma pr1_pack_sigma_eq : ∀ (A : Type) (P : A → Type) (p q : A) (x : P p) (y : P q) (e1 : p = q)
+                            (e2 : rew e1 in x = y), cong pr1 (pack_sigma_eq e1 e2) = e1.
+Proof.
+  intros. destruct e1. destruct e2. simpl. reflexivity.
+Defined.
+
+Lemma sigma_eq_1_pack_sigma_eq : ∀ (A : Type) (P : A → Type) (p q : A) (x : P p) (y : P q) (e1 : p = q)
+                            (e2 : rew e1 in x = y), sigma_eq_1 (pack_sigma_eq e1 e2) = e1.
+Proof.
+  intros. destruct e1. destruct e2. simpl. reflexivity.
+Defined.
+
+Polymorphic Definition pack_sigma_eq_cong {A} {x y : A} (f : A -> A)
+            (e : x = y)
+            {e' : f x = f y}
+            (e'' : cong f e = e') :
+  { a : @sigmaI _ (fun x => f x = f y) x (cong f e) = &(y & eq_refl) &
+    sigma_eq_1 a = e }.
+Proof. destruct e. destruct e''. simpl. exists eq_refl. apply eq_refl. Defined.
+
+Lemma apply_equiv_dom {A B} (P : B -> Type) (e : Equiv A B) :
+  (forall x : A, P (equiv e x)) -> forall x : B, P x.
+Proof.
+  intros. destruct e.
+  specialize (X (equiv_inv x)).
+  rewrite inv_equiv_equiv in X. exact X.
+Defined.
+
+Definition vector_args_type {A} {E} (n : ℕ E) (v : Vec E A n) : Type :=
+  match v with
+  | nil => unit
+  | @cons _ _ n' a v => &{ n : _ & &{a : A & Vec E A n }}
+  end.
+
+Definition vector_args {A} {E} (n : ℕ E) (v : Vec E A n) : vector_args_type n v :=
+  match v as v' in Vec _ _ n return vector_args_type n v' with
+  | nil => tt
+  | @cons _ _ n a v => &(n, a & v)
+  end.
+
+Definition apd {A} {B : A -> Type} (f : forall x : A, B x) {x y : A} (p : x = y) :
+  rew p in f x = f y.
+Proof. destruct p; reflexivity. Defined.
+
 Set Nested Proofs Allowed.
-Equations param_vector_vcons E (A : Set) (a : A) (n : ℕ E) (v : Vec E A n)
+
+(* Definition cong {A B : Type} (f : A -> B) {x y : A} (e : x = y) : f x = f y := *)
+(*   J (fun y _ => f x = f y) (@eq_refl _ (f x)) y e. *)
+
+Inductive sig_eq {A : Type} {B : A -> Type} (x : &{ x : A & B x }) : forall y : &{ x : A & B x }, x = y -> Prop :=
+  sig_eq_refl : sig_eq x x eq_refl.
+
+Inductive is_refl {A : Type} {x : A} : forall {y : A}, x = y -> Prop :=
+  is_refl_refl : is_refl eq_refl.
+
+Lemma is_refl_refl' {A : Type} {x : A} (p : x = x) : is_refl p -> p = eq_refl.
+Proof.
+  intros H.
+  generalize_eqs_sig H.
+  destruct H. simpl.
+  intros.
+  pose (apd (A:=sigma A (fun y : A => x = y)) (fun x => pr2 x) H).
+  simpl in e. rewrite <- e. clear.
+  revert x p H.
+
+  Lemma eq_subst {A} : ∀ (x y : A) (p : x = y) (H : y = y) (prf : eq_refl = H),
+      p = rewP H at (fun y => eq x y) in p.
+  Proof. intros. destruct p. destruct prf. reflexivity. Qed.
+  intros.
+  pose (cong (A:=sigma A (fun y : A => x = y)) (fun x => pr1 x) H).
+  simpl in e.
+Admitted.
+
+Lemma sig_eq_pr1 {A : Type} {B : A -> Type} (x : A) (p : B x) (q : B x)
+      (e : x = x) (e' : rew e in p = q) : sig_eq _ _ (pack_sigma_eq e e') -> e = eq_refl.
+Proof.
+  destruct e'.
+  intros.
+  generalize_eqs_sig H.
+  destruct H. simpl.
+  intros.
+  pose (apd (A:=(sigma (sigma A (fun x : A => B x))
+                       (fun y : sigma A (fun x : A => B x) => @eq (sigma A (fun x : A => B x)) (@sigmaI A B x p) y))
+            ) (fun x => pr2 x) H). simpl in e0.
+  pose (apd (A:=@eq (sigma A (fun x : A => B x)) (@sigmaI A B x p) (@sigmaI A B _ _))
+            (fun x => sigma_eq_1 x) e0).
+  simpl in e1. rewrite <- e1.
+  clear e1.
+  subst e0.
+
+  (* Lemma sigma_eq_1_rew {A : Type} {B : A -> Type} (x : A) (p : B x) (q : B x) *)
+  (*     (e : x = x) (e' : rew e in p = q) (H :  : sigma_eq_1 (rew H in pack_sigma_eq e e'). *)
+Admitted.
+
+Lemma cong_f {A B} (f : A -> B) (g : B -> A)
+      (retr : forall x, g (f x) = x)
+      (x y : A) (e : x = y) (e' : f x = f y) :
+  cong f e = e' -> e = rewP retr x at (fun z => z = y) in (rewP (retr y) at (fun z => g (f x) = z) in cong g e').
+Proof.
+  intros.
+  destruct e. simpl in *.
+  unfold subst_expl. unfold subst.
+  destruct H. simpl. destruct (retr x). simpl. reflexivity.
+Qed.
+
+  Definition eq_fn {A B} (e : A = B) : A -> B.
+    destruct e. exact id.
+  Defined.
+
+(* Lemma apply_eq_dom {A B : Type} (P : B -> Type) (e : A  B) : *)
+(*   (forall x : A, P (eq_fn e x)) -> forall x : B, P x. *)
+(* Proof. *)
+(*   intros. destruct e. apply X. Defined. *)
+
+Lemma cong_f_inj {A B} (f : A -> B) (g : B -> A)
+      (retr : forall x y, f x = f y -> x = y)
+      (x y : A) (e e' : x = y) :
+  cong f e = cong f e' -> e = e'.
+Proof.
+  intros.
+Admitted.
+
+Polymorphic Definition sigma_eq_2'' {A} {B : A -> Type} {x y : &{ x : A & B x }} :
+  forall e : x = y, (@eq_rect A x.1 B x.2 y.1 (cong pr1 e)) = y.2.
+ Proof.
+  destruct e. reflexivity.
+Defined.
+
+Definition vect_hd {A E n} (v : Vec A E (S n)) :=
+  match v with
+  | cons a' v' => a'
+  end.
+
+Definition vect_tl {A E n} (v : Vec A E (S n)) :=
+  match v with
+  | cons a' v' => v'
+  end.
+
+ Equations param_vector_vcons E (A : Set) (a : A) (n : ℕ E) (v : Vec E A n)
           (X : vector_param E A (S n) (cons a v)) : vector_param E A n v :=
   param_vector_vcons E A _ _ _  (vcons_param _ _ _ X) := X.
 Transparent param_vector_vcons.
 Next Obligation.
-  generalize_eqs_sig X. destruct X.
+  generalize_eqs_sig X.
+  destruct X.
   simplify ?. simpl.
-  apply eq_simplification_sigma1_dep.
+  refine (eq_simplification_sigma1_dep_dep _ _ _ _ _).
   refine (eq_simplification_sigma1_dep_dep (S n) (S n0) (cons a v) (cons a0 v0) _).
   simplify ?.
   simplify ?.
-  simpl.
-  refine (simplify_ind_pack _ _ _ _ _ _). simpl.
+  simpl noConfusion_inv.
+  Opaque pack_sigma_eq.
+  change (cons a v) with (rewP (cong S eq_refl) at (fun x => Vec E A x) in (cons a v)).
+  unfold subst_expl.
+  refine (simplify_ind_pack _ _ _ _ _ _ _ _). simpl. unfold opaque_ind_pack_eq_inv.
   simplify ?.
+  set (pack := NoConfusionPackage_Vec E A).
   unfold NoConfusion. unfold NoConfusionPackage_Vec.
   unfold NoConfusion_Vec.
   intros H. simpl in H.
-  unfold noConfusion_inv. unfold noConfusion_Vec_obligation_2.
+  (* assert (∀ (a b : &{ index : ℕ E & Vec E A index}) (e : NoConfusion a b), noConfusion (noConfusion_inv e) = e). *)
+  (* destruct a1, b. destruct pr2, pr3; simpl. intros. *)
+  (* unfold noConfusion_Vec_obligation_1. destruct e. simpl. reflexivity. *)
+  (* intros e. destruct e. *)
+  (* intros e. destruct e. *)
+  (* intros e. *)
+  (* unfold noConfusion_Vec_obligation_1. destruct e. simpl. reflexivity. *)
+  (* specialize (H0 &(S n0 & cons a v) &(S n0 & cons a0 v0) H). *)
+  (* apply (cong (cong cf)) in H0. *)
+
+  unfold noConfusion_inv. simpl.
+  unfold noConfusion_Vec_obligation_2.
   change (match
              H in (_ = y)
              return (&(S n0 & cons a v) = &(S y.(pr1) & cons y.(pr2).(pr1) y.(pr2).(pr2)))
            with
            | eq_refl => eq_refl
-           end) with (f_equal (fun x => &(S x.1 & cons x.2.1 x.2.2)) H).
+           end) with (cong (fun x => &(S x.1 & cons x.2.1 x.2.2)) H).
+  (* remember ((cong (λ x : &{ n : ℕ E & &{ _ : A & Vec E A n}}, &(S x.(pr1) & cons x.(pr2).(pr1) x.(pr2).(pr2))) H)) as e'. *)
+  (* simpl in e'. *)
+ set(cf := (λ x : &{ n : ℕ E & &{ _ : A & Vec E A n}}, &(S x.(pr1) & cons x.(pr2).(pr1) x.(pr2).(pr2)))).
+  revert H.
+  refine (eq_simplification_sigma1_dep_dep _ _ _ _ _).
+  intros.
+  revert e0.
+  revert ee.
+  intros ee.
+
+  revert ee.
+
+
+  unshelve evar(x : (@eq_refl _ (S n0)) = (cong (fun x => S x) e')).
+  { rewrite <- ee.
+    rewrite (cong_iter cf pr1 _ _ (pack_sigma_eq e' e)).
+    subst cf. simpl.
+    rewrite <- (cong_iter pr1 (fun x => S x) _ _ (pack_sigma_eq e' e)).
+    rewrite pr1_pack_sigma_eq. reflexivity. }
+  exact H. subst x.
+
+  set (g := (fun x => match x return ℕ E with S x => x | _ => x end)).
+  unshelve evar(retr : forall x, g (S x) = x).
+  intros. unfold g. reflexivity.
+  symmetry in X1. eapply (cong_f S g retr) in X1.
+  subst retr. simpl in X1. subst e'.
+  revert ee. simpl. simpl in e.
+  revert e.
+  simplify ?. simpl.
+  simplify ?. simpl.
+
+
+  refine (apply_equiv_dom _ He _).
+  intros x. destruct x.
+  simpl.
+
+  apply cheat. Defined.
+  simplify ?. simpl.
+  simplify ?. simpl.
+  constructor.
+Defined.
+
+  unfold ind_pack_eq_inv. unfold sigma_eq_2'.
+  unfold
+
+  pose proof (eq_sym (cong_iter cf pr1 _ _ match e in (_ = y) return (&(n0, a & v) = &(n0 & y)) with
+                                           | eq_refl => eq_refl
+                                           end)).
+
+  refine (@apply_equiv_dom (cong (λ x : &{ n : ℕ E & &{ _ : A & Vec E A n}}, (cf x).1)
+        match e in (_ = y) return (&(n0, a & v) = &(n0 & y)) with
+        | eq_refl => eq_refl
+        end) _ H _).
+
+
+
+
+  rewrite H0 in ee.
+  specialize (f_equal_inv' (fun x => (cf x).1) (fun _ : &{ n : ℕ E & &{ _ : A & Vec E A n}} => S n0)
+                           &(n0, a & v) &(n0, a0 & v0) eq_refl eq_refl H ee).
+  simpl. unfold subst_expl. subst cf. simpl.
+  simpl in *.
+  intros. apply H1.
+  subst x.
+  revert H ee X1. subst cf.
+  intros H ee X1. revert ee.
+  unfold ind_pack_eq_inv.
+  revert H X1.
+  refine (eq_simplification_sigma1_dep_dep _ _ _ _ _).
+  intros.
+
+  Lemma rew_cong {A B} (f : A -> B) (x y : A) (e : x = y)  : (rew cong f e in (@eq_refl B (f x))) = cong f e.
+  Proof. destruct e. reflexivity. Defined.
+
+  pose proof (rew_cong (λ x : &{ n : ℕ E & &{ _ : A & Vec E A n}}, S x.(pr1)) _ _ (pack_sigma_eq e' e)).
+  simpl in H0.
+  revert X1.
+  match goal with
+    |- ?X =_{_;_} _ -> _ => set (foo:=X)
+  end.
+  replace foo
+    with (cong (λ x : &{ n : ℕ E & &{ _ : A & Vec E A n}}, S x.(pr1)) (pack_sigma_eq e' e)).
+  intros.
+  2:{ subst foo. rewrite <- H0 at 1. admit. }
+
+
+
+  subst cf.
+  assert (&{n : ℕ E & &{ _ : A & &{ _ : Vec E A n0 & S n = S n}}} <~>
+          &{n : ℕ E & &{ _ : A & &{ _ : Vec E A n0 & S n0 = S n0}}}).
+  unshelve econstructor. intros [n [a' [v' e']]]. exists n. exists a. exists v'. reflexivity.
+  unshelve econstructor. intros [n [a' [v' e']]]. exists n. exists a. exists v'. reflexivity.
+  red. intros [n [a' [v' e']]]. admit. admit. admit.
+  pose proof (is_equiv _ _ X2).
+  pose (@isEquiv_cong _ _ _ X2 &(n0, a, v & eq_refl) &(n0, a0 , v0 & eq_refl)).
+  pose (f_equal X2 (x:=&(n0, a0, v0 & eq_refl)) (y:=&(n0, a0, v0 & eq_refl))).
+  pose (@isequiv _ _ _ i). simpl in e.
+
+
+
+  destruct (pack_sigma_eq_cong _ e' ee). as [e'0 ee'0]. revert ee'.
+
+  destruct ee'0.
+  unshelve evar (equi : &{ x : ℕ E & S x = S n0} <~> ()).
+  unshelve econstructor. exact (fun _ => tt). unshelve econstructor.
+  intros. exists n0. reflexivity. red. destruct x. auto.
+  red. intros [x Heq]. revert Heq. simplify *. reflexivity.
+  admit.
+  revert e'0.
+  epose (apply_equiv_dom _ (equiv_sym e)).
+  refine (y _). simpl.
+  intros Hx. clear y.
+  assert (sigma_eq_1 (inv_equiv e Hx) = eq_refl).
+  subst e.
+  unfold Equiv_cong. simpl. unfold inv_equiv.
+  unfold equiv_inv;simpl.
+  unfold sigma_eq_1. simpl. unfold pack_sigma_eq. simpl.
+  unfold eq_ind. simpl. unfold apply_noConfusion. simpl.
+  unfold noConfusion_ℕ_obligation_3. simpl.
+  unfold noConfusion_ℕ_obligation_1. simpl.
+  unfold cong. simpl.
+  unfold inv_equiv_equiv
+
+
+
+
+
+  simpl.
+  simpl.
+  specialize (i &(n0 & cong S e') &(n0 & eq_refl)).
+  revert i.
+  match goal with
+  pattern (f_equal _). (λ _ : &{ x : ℕ E & S x = S n0}, ())
+                                (x := &(n0 & cong (λ x : ℕ E, S x) e'))
+                                (y:=&(n0 & eq_refl))).
+  destruct i. pose (equiv_inv0 eq_refl).
+  red in eissect0.
+
+
+
+
+
+
+  change eq_refl with (cong (fun x => S x) (@eq_refl _ n0)) in ee'.
+  unfold subst_expl in e0. simpl in e0. simpl in ee'.
+  eq_refl eq_refl e'). simpl in e0.
+  (* eq_refl (cong (fun x : ℕ E => S x) e') eq_refl eq_refl). *)
+  simpl in e0. unfold subst_expl in e0.
+  rewrite cong_p
+
+  simpl in ee'.
+
+  rewrite
+
+
+
+  pose (f_equal_inv_pack (A := ℕ E)
+                               (fun x => S x)
+                               (fun x => S x)).
+  simpl in e. specialize (e &(n0 & eq_refl)).
+  simpl in e.
+  intros H.
+  unshelve epose proof (e &(n0 & _)).
+  simpl. exact (cong
+                                  (λ j : &{ n : ℕ E & &{ _ : A & Vec E A n}},
+                                         (S j.(pr1))) H).
+  simpl in H0. specialize (H0 eq_refl). simpl in *.
+
+  forward H0.
+  unfold subst_expl.
+
+  simpl in H0.
+
+
+  pose (f_equal_inv_pack (A := &{ n0 : _ & &{ a : A & Vec E A n0 }})
+                               (fun x => S x.1)
+                               (fun x => S x.1)).
+  simpl in e. specialize (e &( &(n0, a & v) & eq_refl)).
+  simpl in e.
+  intros H.
+  unshelve epose proof (e &(&(n0, a0 & v0) & _)).
+  simpl. exact (cong
+                                  (λ j : &{ n : ℕ E & &{ _ : A & Vec E A n}},
+                                         (S j.(pr1))) H).
+  simpl in H0. specialize (H0 H). clear e.
+  forward H0.
+  unfold subst_expl.
+
+  simpl in H0.
+
+                         )).
+  refine pack_f_equal.
+
+
   assert (f_equal pr1
            (f_equal
               (fun x : &{ n : ℕ E & &{ _ : A & Vec E A n}} =>
@@ -345,80 +895,20 @@ Next Obligation.
   revert H H'.
   intros H.
   change (@eq_refl _ (S n0)) with (f_equal (fun x : &{ n : ℕ E & &{ _ : A & Vec E A n}} => S x.1) (@eq_refl _ &(n0, a & v))) at 1.
-
-
-Polymorphic
-Definition sigma_eq_2_f  {A A'} {B : A' -> Type} {f : A -> A'} {x y : &{ x : A & B (f x) }} : (x = y) -> (&(f x.1 & x.2) = &(f y.1 & y.2)).
-Proof.
-  destruct x, y. simpl.
-  intros H.
-  apply sigma_eq_decomp. simpl.
-  apply sigma_eq_decomp_inv in H as [H1 H2]. simpl in *.
-  exists (f_equal f H1). simpl. destruct H1. simpl in *. exact H2.
-Defined.
-
-Definition sigma_eq_2_f_inv  {A A'} {B : A' -> Type} {f : A -> A'}
-           {fequiv : IsEquiv f}
-           {x y : &{ x : A & B (f x) }} : (&(f x.1 & x.2) = &(f y.1 & y.2)) -> (x = y).
-Proof.
-  intros. apply sigma_eq_decomp_inv in H.
-  apply sigma_eq_decomp. simpl in *. destruct H.
-  revert pr2.
-  pose proof (isEquiv_cong f fequiv x.1 y.1).
-  simpl in *. pose proof (eisretr (IsEquiv := H) pr1).
-  rewrite <- H0.
-  exists (equiv_inv pr1). clear -pr2.
-  revert pr2.
-  generalize (equiv_inv pr1). destruct y.
-  simpl. intros <-. trivial.
-Defined.
-
-Polymorphic
-  Lemma f_equal_inv {A} {B : Type} (a b : A -> B) (u v : A)
-        (F : &{ x : A & a x = b x } -> Type)
-        (r : a u = b u)
-        (s : a v = b v)
-        (e : u = v)
-        (e' : eq_trans (eq_sym r) (eq_trans (f_equal a e : a u = a v) s) = f_equal b e) :
-    (F &(u & r) = F &(v & s)).
-  Proof.
-    intros.
-    pose (@f_equal _ _ F &(u & r) &(v & s)). apply e0. clear e0.
-
-    pose (@make_sigma_eq A (fun x => b u = b x) u v). simpl in e0.
-    specialize (e0 (eq_trans (eq_sym r) (eq_trans (f_equal a e) (eq_trans s (f_equal b (eq_sym e))))) (f_equal b e) e). forward e0. apply cheat.
-    apply (sigma_eq_2_f (f := fun x => b x)) in e0.
-    simpl in *.
-
-
-    pose proof (sigma_eq_2_cong
-                  (A := A) (A' := B) (B := fun y :  => @eq B (a y) (b y))
-                  (x := &(u & r)) (y := &(v & s)) (f := fun x : A => a x)
-               ). simpl in H.
-
-    aply forward e0.
+  revert H.
 
 
 
-    destruct s. unfold eq_trans, eq specialize (H x y).
-    destruct p. simpl in *. apply
-
-
-  Lemma pack_f_equal {A} {B : A -> Type} (x : A) (p q : B x) (f : A -> A)
-        (G : forall (e : &(x & p) = &(x & q)) (e' : eq_refl = f_equal (fun x => f x.1) e), Type) :
-    (forall (e : &(x & p) = &(x & q))
-            (e' : f_equal (fun x => f x.1) eq_refl = f_equal (fun x => f x.1) e), G e e') ->
-    (forall (e : &(x & p) = &(x & q)) (e' : eq_refl = f_equal (fun x => f x.1) e), G e e').
-  Proof. intros. simpl in *. apply X. Defined.
-  refine (pack_f_equal _ _ _ _ _ _ _).
 
   unfold opaque_ind_pack_eq_inv.
-  simpl in *.
+
 
 
   pose (sigma_eq_1_f_equal   &(n0, a & v) &(n0, a0 & v0) (fun x => S x) (fun x => cons x.2.1 x.2.2) H).
   simpl in e. symmetry in e.
   refine (rewrite_prod e _).
+
+
 
 
   unfold f_equal at 2. simpl
